validate_bounded_strong_prefix (remove validator_max_length slice precond)

src/lowparse/LowParse.Low.Base.fst
@@ -2099,6 +2099,60 @@ let validator (#k: parser_kind) (#t: Type) (p: parser k t) : Tot Type =
   )))
 
 inline_for_extraction
+let validate_bounded_strong_prefix
+  (#k: parser_kind) (#t: Type) (#p: parser k t)
+  (v: validator p)
+  (#rrel: _) (#rel: _)
+  (sl: slice rrel rel)
+: HST.Stack U32.t
+  (requires (fun h ->
+    live_slice h sl /\
+    Some? k.parser_kind_high /\
+    Some?.v k.parser_kind_high <= U32.v validator_max_length /\
+    k.parser_kind_subkind == Some ParserStrong
+  ))
+  (ensures (fun h res h' ->
+    B.modifies B.loc_none h h' /\ (
+    if U32.v res <= U32.v validator_max_length
+    then
+      valid_pos p h sl 0ul res
+    else
+      (~ (valid p h sl 0ul))
+  )))
+= if sl.len `U32.lte` validator_max_length
+  then v sl 0ul
+  else
+    let h = HST.get () in
+    let sl' = make_slice sl.base validator_max_length in
+    let res = v sl' 0ul in
+    let phi () : Lemma
+      (ensures (
+        if U32.v res <= U32.v validator_max_length
+        then
+          valid_pos p h sl 0ul res
+        else
+          (~ (valid p h sl 0ul))
+      ))
+    =
+      valid_facts p h sl 0ul;
+      valid_facts p h sl' 0ul;
+      if U32.v res <= U32.v validator_max_length
+      then
+        parse_strong_prefix p (bytes_of_slice_from h sl' 0ul) (bytes_of_slice_from h sl 0ul)
+      else
+        let psi () : Lemma
+          (requires (valid p h sl 0ul))
+          (ensures False)
+        = let len = get_valid_pos p h sl 0ul in
+          assert (U32.v len <= U32.v validator_max_length);
+          parse_strong_prefix p (bytes_of_slice_from h sl 0ul) (bytes_of_slice_from h sl' 0ul)
+        in
+        Classical.move_requires psi ()
+    in
+    let _ = phi () in
+    res
+
+inline_for_extraction
 let validate
   (#k: parser_kind)
   (#t: Type)
